Sodium/Crypto/Box.lean
@@ -1,0 +1,74 @@
+import Sodium.Theory.Basic
+import Sodium.Data.Aead
+import Sodium.Data.Curve25519
+import Sodium.Data.Ristretto255
+import Sodium.Data.Core
+
+namespace Sodium.Crypto
+
+open Sodium.Theory
+
+def xsalsa20poly1305 : Aead where
+  name := `xsalsa20poly1305
+  keyBytes := 32
+  nonceBytes := 24
+  tagBytes := 16
+  encrypt := XSalsa20Poly1305.encrypt
+  decrypt? := XSalsa20Poly1305.decrypt?
+
+def xchacha20poly1305 : Aead where
+  name := `xchacha20poly1305
+  keyBytes := 32
+  nonceBytes := 24
+  tagBytes := 16
+  encrypt := XChaCha20Poly1305.encrypt
+  decrypt? := XChaCha20Poly1305.decrypt?
+
+def aegis256 : Aead where
+  name := `aegis256
+  keyBytes := 32
+  nonceBytes := 32
+  tagBytes := 32
+  encrypt := Aegis256.encrypt
+  decrypt? := Aegis256.decrypt?
+
+def curve25519 : DhFunction where
+  name := `curve25519
+  scalarBytes := 32
+  pointBytes := 32
+  mulBase := Curve25519.mulBase
+  mul := Curve25519.mul
+
+def ristretto255Order : Nat := 2 ^ 252 + 27742317777372353535851937790883648493
+
+def ristretto255 : PrimeOrderGroup where
+  name := `ristretto255
+  scalarBytes := 32
+  pointBytes := 32
+  uniformBytes := 64
+  nonReducedBytes := 64
+  mulBase := Ristretto255.mulBase
+  mul := Ristretto255.mul
+  add := Ristretto255.add
+  sub := Ristretto255.sub
+  fromUniform := Ristretto255.fromHash
+  validPoint := Ristretto255.isValidPoint
+  scalarReduced s :=
+    decide (s.toByteArray.toList.foldr (fun b acc => b.toNat + 256 * acc) 0 < ristretto255Order)
+  scalarReduce := Ristretto255.scalarReduce
+  scalarAdd := Ristretto255.scalarAdd
+  scalarMul := Ristretto255.scalarMul
+  scalarNeg := Ristretto255.scalarNeg
+
+theorem curve25519_lawful : curve25519.Lawful := sorry
+theorem ristretto255_lawful : ristretto255.Lawful := sorry
+theorem xsalsa20poly1305_lawful : xsalsa20poly1305.Lawful := sorry
+
+def box : Box := dhBox curve25519 xsalsa20poly1305 hsalsa20
+def boxXchacha20poly1305 : Box := dhBox curve25519 xchacha20poly1305 hchacha20
+def boxRistretto255 : Box := dhBox ristretto255.toDhFunction xchacha20poly1305 blake2b32
+
+theorem box_lawful : box.Lawful :=
+  dhBox_lawful curve25519 xsalsa20poly1305 hsalsa20 curve25519_lawful xsalsa20poly1305_lawful
+
+end Sodium.Crypto
